aneris/examples/reliable_communication/lib/repdb/proof/leader/followers_mt_user_params.v
@@ -58,7 +58,6 @@ Section MT_user_params.
       MTS_rep_ser_inj_alt := rep_l2f_ser_is_injective_alt;
       MTS_rep_data := RepData;
       MTS_saddr := DB_addrF;
-      MTS_mN := (DB_InvName .@ "leader_secondary");
       MTS_handler_pre  := ReqPre;
       MTS_handler_post := ReqPost;
     |}.
